hit a snag thinking again.

theories/RTac/Core.v
@@ -13,6 +13,7 @@ Require Import ExtLib.Tactics.
 Require Import MirrorCore.ExprI.
 Require Import MirrorCore.SubstI.
 Require Import MirrorCore.ExprDAs.
+Require Import MirrorCore.RTac.Ctx.
 
 Require Import MirrorCore.Util.Quant.
 Require Import MirrorCore.Util.Forwardy.
@@ -51,38 +52,50 @@ Ltac equivs :=
 Section parameterized.
   Variable typ : Type.
   Variable expr : Type.
-  Variable subst : Type.
 
   Context {RType_typ : RType typ}.
   Context {Expr_expr : Expr RType_typ expr}.
   Context {ExprOk_expr : ExprOk Expr_expr}.
   Context {Typ0_Prop : Typ0 _ Prop}.
-  Context {Subst_subst : Subst subst expr}.
-  Context {SubstOk_subst : @SubstOk _ _ _ _ Expr_expr Subst_subst}.
-  Context {SubstUpdate_subst : SubstUpdate subst expr}.
-  Context {SubstUpdateOk_subst : @SubstUpdateOk _ _ _ _ Expr_expr Subst_subst _ _}.
-  Context {SubstInstantiatable_subst : SubstInstantiatable subst expr}.
-  Context {SubstInstantiatableOk_subst : @SubstInstantiatableOk _ _ _ _ Expr_expr Subst_subst _ _}.
+
+  Variable instantiate : (nat -> option expr) -> nat -> expr -> expr.
+
+  Local Notation "'rsubst'" := (FMapSubst.SUBST.raw expr) (at level 0).
 
   Inductive Goal :=
   | GAll    : typ -> Goal -> Goal
-  (** The first element in the list has the lowest index
-   ** in the final goal.
-   **)
-  | GExs    : list (typ * option expr) -> Goal -> Goal
+  | GExs    : list typ -> rsubst -> Goal -> Goal
   | GHyp    : expr -> Goal -> Goal
   | GConj_  : Goal -> Goal -> Goal
   | GGoal   : expr -> Goal
   | GSolved : Goal.
 
+  Inductive WellFormed_Goal (tus tvs : tenv typ) : Goal -> Prop :=
+  | WFExs : forall ts s g,
+              FMapSubst.SUBST.WellFormed s ->
+              only_in_range (length tus) (length ts) s ->
+              WellFormed_Goal (tus ++ ts) tvs g ->
+              WellFormed_Goal tus tvs (GExs ts s g)
+  | WFAll : forall t g, WellFormed_Goal tus (tvs ++ t :: nil) g ->
+                        WellFormed_Goal tus tvs (GAll t g)
+  | WFHyp : forall t g, WellFormed_Goal tus tvs g ->
+                        WellFormed_Goal tus tvs (GHyp t g)
+  | WFConj_ : forall g1 g2, WellFormed_Goal tus tvs g1 ->
+                            WellFormed_Goal tus tvs g2 ->
+                            WellFormed_Goal tus tvs (GConj_ g1 g2)
+  | WFGoal : forall g, WellFormed_Goal tus tvs (GGoal g)
+  | WFSovled : WellFormed_Goal tus tvs GSolved.
+
   Definition GAlls (ts : list typ) (g : Goal) : Goal :=
     fold_right (fun x y => GAll x y) g ts.
 
+(*
   Definition GEx (t : typ) (e : option expr) (g : Goal) : Goal :=
     match g with
       | GExs tes g' => GExs ((t,e) :: tes) g'
       | _ => GExs ((t, e) :: nil) g
     end.
+*)
 
   Definition GConj l r : Goal :=
     match l with
@@ -110,398 +123,15 @@ Section parameterized.
                    end
     end.
 
-  Inductive Ctx :=
-  | CTop
-  | CAll : Ctx -> typ -> Ctx
-  | CExs : Ctx -> list typ -> Ctx
-  | CHyp : Ctx -> expr -> Ctx.
-
-  Fixpoint CEx (c : Ctx) (t : typ) : Ctx :=
-    CExs c (t :: nil).
-
-  Fixpoint CAlls (c : Ctx) (ls : list typ) : Ctx :=
-    match ls with
-      | nil => c
-      | l :: ls => CAlls (CAll c l) ls
-    end.
-
-  (** Auxiliary Functions **)
-  Fixpoint countVars (ctx : Ctx) : nat :=
-    match ctx with
-      | CTop => 0
-      | CAll ctx' t => S (countVars ctx')
-      | CExs ctx' _
-      | CHyp ctx' _ => countVars ctx'
-    end.
-
-  Fixpoint countUVars (ctx : Ctx) : nat :=
-    match ctx with
-      | CTop => 0
-      | CExs ctx' ts => length ts + countUVars ctx'
-      | CAll ctx' _
-      | CHyp ctx' _ => countUVars ctx'
-    end.
-
-  Fixpoint getUVars (ctx : Ctx) : tenv typ :=
-    match ctx with
-      | CTop => nil
-      | CAll ctx' _ => getUVars ctx'
-      | CExs ctx' ts => getUVars ctx' ++ ts
-      | CHyp ctx' _ => getUVars ctx'
-    end.
-
-  Fixpoint getVars (ctx : Ctx) : tenv typ :=
-    match ctx with
-      | CTop => nil
-      | CAll ctx' t => getVars ctx' ++ t :: nil
-      | CExs ctx' _ => getVars ctx'
-      | CHyp ctx' _ => getVars ctx'
-    end.
-
-  Lemma countVars_getVars : forall ctx, countVars ctx = length (getVars ctx).
-    induction ctx; simpl; auto.
-    rewrite app_length. simpl. omega.
-  Qed.
-
-  Lemma countUVars_getUVars : forall ctx, countUVars ctx = length (getUVars ctx).
-    induction ctx; simpl; auto.
-    rewrite app_length. simpl. omega.
-  Qed.
-
-  Fixpoint getEnvs' (ctx : Ctx) (tus tvs : tenv typ)
-  : tenv typ * tenv typ :=
-    match ctx with
-      | CTop => (tus,tvs)
-      | CAll ctx' t => getEnvs' ctx' tus (t :: tvs)
-      | CExs ctx' ts => getEnvs' ctx' (ts ++ tus) tvs (** TODO: Check **)
-      | CHyp ctx' _ => getEnvs' ctx' tus tvs
-    end.
-
-  Definition getEnvs (ctx : Ctx) : tenv typ * tenv typ :=
-    let (x,y) := getEnvs' ctx nil nil in
-    (x, y).
-
-  Fixpoint Ctx_append (c1 c2 : Ctx) : Ctx :=
-    match c2 with
-      | CTop => c1
-      | CAll ctx' t => CAll (Ctx_append c1 ctx') t
-      | CExs ctx' ts => CExs (Ctx_append c1 ctx') ts
-      | CHyp ctx' h => CHyp (Ctx_append c1 ctx') h
-    end.
-
-  Theorem getUVars_append
-  : forall c1 c2,
-      getUVars (Ctx_append c1 c2) = getUVars c1 ++ getUVars c2.
-  Proof.
-    clear. induction c2; simpl; eauto.
-    symmetry; eapply app_nil_r_trans.
-    rewrite IHc2. apply app_ass_trans.
-  Defined.
-
-  Theorem getVars_append
-  : forall c1 c2,
-      getVars (Ctx_append c1 c2) = getVars c1 ++ getVars c2.
-  Proof.
-    clear. induction c2; simpl; eauto.
-    symmetry; eapply app_nil_r_trans.
-    rewrite IHc2. apply app_ass_trans.
-  Defined.
-  (** End: Auxiliary Functions **)
-
-  Inductive ctx_subst : Ctx -> Type :=
-  | TopSubst : subst -> ctx_subst CTop
-  | AllSubst : forall {t c}, ctx_subst c -> ctx_subst (CAll c t)
-  | HypSubst : forall {t c}, ctx_subst c -> ctx_subst (CHyp c t)
-  | ExsSubst : forall {ts c}, ctx_subst c -> subst -> ctx_subst (CExs c ts).
-
-  Definition only_in_range (min len : nat) (s : subst) : Prop :=
-    forall u e, subst_lookup u s = Some e -> min <= u < min + len.
-
-  Inductive WellFormed_ctx_subst : forall c, ctx_subst c -> Prop :=
-  | WF_TopSubst : forall s,
-                    WellFormed_subst s ->
-                    only_in_range 0 0 s -> (** eeks **)
-                    WellFormed_ctx_subst (TopSubst s)
-  | WF_AllSubst : forall t c s,
-                    WellFormed_ctx_subst s ->
-                    WellFormed_ctx_subst (@AllSubst t c s)
-  | WF_HypSubst : forall t c s,
-                    WellFormed_ctx_subst s ->
-                    WellFormed_ctx_subst (@HypSubst t c s)
-  | WF_ExsSubst : forall t c s s',
-                    WellFormed_subst s' ->
-                    only_in_range (countUVars c) (length t) s' ->
-                    WellFormed_ctx_subst s ->
-                    WellFormed_ctx_subst (@ExsSubst t c s s').
-
-  Fixpoint ctx_lookup {c} (u : nat) (cs : ctx_subst c) : option expr :=
-    match cs with
-      | TopSubst s => subst_lookup u s
-      | AllSubst _ _ c => ctx_lookup u c
-      | HypSubst _ _ c => ctx_lookup u c
-      | ExsSubst _ _ c s =>
-        match subst_lookup u s with
-          | None => ctx_lookup u c
-          | Some e => Some e
-        end
-    end.
-
-  Fixpoint ctx_domain {c} (cs : ctx_subst c) : list nat :=
-    match cs with
-      | TopSubst s => subst_domain s
-      | AllSubst _ _ c => ctx_domain c
-      | HypSubst _ _ c => ctx_domain c
-      | ExsSubst _ _ c s =>
-        ctx_domain c ++ subst_domain s
-    end.
-
-  Fixpoint all_convertible (xs ys : tenv typ) : bool :=
-    match xs , ys with
-      | nil , nil => true
-      | x :: xs , y :: ys =>
-        match type_cast x y with
-          | None => false
-          | Some _ => all_convertible xs ys
-        end
-      | _ , _ => false
-    end.
-
-  Theorem all_convertible_sound
-  : forall xs ys,
-      all_convertible xs ys = true -> xs = ys.
-  Proof.
-    induction xs; destruct ys; simpl; intros; try congruence.
-    destruct (type_cast a t).
-    { destruct r. f_equal; eauto. }
-    { congruence. }
-  Qed.
-
-  Definition drop_exact (tus ts : tenv typ)
-  : option { ts' : tenv typ & hlist typD tus -> hlist typD ts' } :=
-    let rem_len := length tus - length ts in
-    let x := skipn rem_len tus in
-    if all_convertible x ts then
-      Some (@existT _ (fun ts' => hlist typD tus -> hlist typD ts')
-                    (firstn rem_len tus)
-                    (fun x =>
-                       fst (hlist_split
-                              (firstn rem_len tus)
-                              (skipn rem_len tus)
-                              match eq_sym (firstn_skipn _ _) in _ = l
-                                    return hlist _ l with
-                                | eq_refl => x
-                              end)))
-    else
-      None.
-
-  Fixpoint ctx_substD {c} tus tvs (cs : ctx_subst c) {struct cs}
-  : option (exprT tus tvs Prop) :=
-    match cs with
-      | TopSubst s => substD tus tvs s
-      | HypSubst _ _ c => ctx_substD tus tvs c
-      | AllSubst t _ c =>
-        match drop_exact tvs (t :: nil) with
-          | None => None
-          | Some (existT tvs' get) =>
-            match ctx_substD tus tvs' c with
-              | None => None
-              | Some sD => Some (fun us vs => sD us (get vs))
-            end
-        end
-      | ExsSubst ts _ c s =>
-        match drop_exact tus ts with
-          | None => None
-          | Some (existT tus' get) =>
-            match substD tus tvs s
-                , ctx_substD tus' tvs c
-            with
-              | Some sD' , Some sD =>
-                Some (fun us vs => sD' us vs /\ sD (get us) vs)
-              | None , _ => None
-              | Some _ , None => None
-            end
-        end
-    end.
-
-  Section ctx_set'.
-    Variables (u : nat) (e : expr) (min : nat) (nus : nat).
-
-    Fixpoint ctx_set' {c T} (cs : ctx_subst c) {struct cs}
-    : ((nat -> option expr) -> ctx_subst c -> option T) -> option T :=
-      match cs in ctx_subst c
-            return ((nat -> option expr) -> ctx_subst c -> option T) -> option T
-      with
-        | TopSubst s => fun k =>
-          match subst_set u e s with
-            | None => None
-            | Some s' =>
-              match subst_lookup u s with
-                | None => None
-                | Some e' => k (fun x => if x ?[ eq ] u then Some e' else None)
-                               (TopSubst s')
-              end
-          end
-        | AllSubst _ _ c => fun k =>
-          ctx_set' c (fun f c => k f (AllSubst c))
-        | HypSubst _ _ c => fun k =>
-          ctx_set' c (fun f c => k f (HypSubst c))
-        | ExsSubst _ ctx c s => fun k =>
-          if u ?[ ge ] (countUVars ctx + nus) then
-            match subst_set u e s with
-              | None => None
-              | Some s' =>
-                match subst_lookup u s with
-                  | None => None
-                  | Some e' =>
-                    k (fun x => if x ?[ eq ] u then Some e' else None)
-                      (ExsSubst c s')
-                end
-            end
-          else
-            ctx_set' c
-                     (fun f c => k f (@ExsSubst _ ctx c
-                                                (subst_instantiate f s)))
-      end.
-  End ctx_set'.
-
-  Definition ctx_set {c} (u : nat) (e : expr) (cs : ctx_subst c)
-  : option (ctx_subst c) :=
-    ctx_set' u e 0 cs (fun _ => @Some _).
-
-  Fixpoint ctx_empty {c} : ctx_subst c :=
-    match c with
-      | CTop => TopSubst (@subst_empty _ _ _)
-      | CHyp c h => HypSubst ctx_empty
-      | CAll c h => AllSubst ctx_empty
-      | CExs c h => ExsSubst ctx_empty (@subst_empty _ _ _)
-    end.
-
-  Global Instance Subst_ctx_subst ctx : Subst (ctx_subst ctx) expr :=
-  { subst_lookup := ctx_lookup
-  ; subst_domain := ctx_domain
-  }.
-
-  Lemma drop_exact_sound
-  : forall tus ts tus' cast,
-      drop_exact tus ts = Some (@existT _ _ tus' cast) ->
-      exists pf : tus' ++ ts = tus,
-        forall a b, cast match pf in _ = tus return hlist _ tus with
-                           | eq_refl => hlist_app a b
-                         end = a.
-  Proof.
-    clear. unfold drop_exact. intros.
-    forward; inv_all; subst.
-    subst.
-    eapply all_convertible_sound in H.
-    exists (match H in _ = z return firstn _ tus ++ z = tus with
-              | eq_refl => firstn_skipn _ _
-            end).
-    intros.
-    generalize (firstn_skipn (length tus - length ts) tus).
-    generalize dependent (skipn (length tus - length ts) tus).
-    generalize dependent (firstn (length tus - length ts) tus).
-    intros; subst. simpl. rewrite hlist_split_hlist_app.
-    reflexivity.
-  Qed.
-
-  Theorem ctx_substD_lookup ctx
-  : forall (s : ctx_subst ctx) (uv : nat) (e : expr),
-      WellFormed_ctx_subst s ->
-      subst_lookup uv s = Some e ->
-      forall (tus tvs : tenv typ) (sD : exprT tus tvs Prop),
-        ctx_substD tus tvs s = Some sD ->
-        exists (t : typ) (val : exprT tus tvs (typD t))
-               (get : hlist typD tus -> typD t),
-          nth_error_get_hlist_nth typD tus uv =
-          Some (existT (fun t0 : typ => hlist typD tus -> typD t0) t get) /\
-          exprD' tus tvs e t = Some val /\
-          (forall (us : hlist typD tus) (vs : hlist typD tvs),
-             sD us vs -> get us = val us vs).
-  Proof.
-    induction 1; simpl; intros.
-    { eapply substD_lookup in H1; eauto. }
-    { forward; inv_all; subst.
-      eapply IHWellFormed_ctx_subst in H3; eauto.
-      forward_reason.
-      exists x0.
-      eapply drop_exact_sound in H2.
-      forward_reason.
-      revert H2.
-      eapply exprD'_weakenV with (tvs' := t :: nil) in H3; eauto.
-      subst tvs.
-      intros. forward_reason.
-      do 2 eexists; split; eauto.
-      split; eauto.
-      intros. erewrite H4; clear H4; eauto.
-      rewrite <- (hlist_app_hlist_split _ _ vs).
-      rewrite <- H5. rewrite H2. reflexivity. }
-    { eauto. }
-    { forward; inv_all; subst.
-      consider (subst_lookup uv s'); intros; inv_all; subst.
-      { eapply substD_lookup in H2; eauto.
-        forward_reason.
-        do 3 eexists; split; eauto. split; eauto.
-        intros. destruct H8. eauto. }
-      { eapply IHWellFormed_ctx_subst in H3; eauto.
-        forward_reason.
-        eapply drop_exact_sound in H4.
-        forward_reason.
-        revert H4. subst tus; intros.
-        exists x0.
-        eapply nth_error_get_hlist_nth_weaken with (ls' := t) in H3.
-        simpl in *. forward_reason.
-        eapply exprD'_weakenU with (tus' := t) in H7; eauto.
-        forward_reason.
-        do 2 eexists; split; eauto; split; eauto.
-        do 2 intro.
-        rewrite <- (hlist_app_hlist_split _ _ us).
-        rewrite <- H9; clear H9.
-        rewrite <- H10; clear H10. destruct 1.
-        eapply H8. rewrite H4 in H10. assumption. } }
-  Qed.
-
-  Lemma ctx_subst_domain ctx
-  : forall (s : ctx_subst ctx),
-      WellFormed_ctx_subst s ->
-      forall (ls : list nat),
-      subst_domain s = ls ->
-      forall n : nat, In n ls <-> subst_lookup n s <> None.
-  Proof.
-    induction 1; simpl; intros; eauto using WellFormed_domain.
-    { subst. rewrite in_app_iff.
-      split; intro.
-      { forward.
-        destruct H2.
-        { eapply IHWellFormed_ctx_subst in H2; eauto. }
-        { eapply WellFormed_domain in H2; eauto. } }
-      { rewrite IHWellFormed_ctx_subst; eauto.
-        rewrite WellFormed_domain; eauto.
-        destruct (subst_lookup n s'); eauto. } }
-  Qed.
-
-  Global Instance SubstOk_cxt_subst ctx
-  : @SubstOk (ctx_subst ctx) typ expr _ _ _ :=
-  { WellFormed_subst := @WellFormed_ctx_subst ctx
-  ; substD := @ctx_substD _
-  }.
-  { eapply ctx_substD_lookup. }
-  { intros; eapply ctx_subst_domain; eauto. }
-  { admit. }
-  Defined.
-
-  Global Instance SubstUpdate_ctx_subst ctx
-  : SubstUpdate (ctx_subst ctx) expr :=
-  { subst_set := ctx_set
-  ; subst_empty := ctx_empty
-  }.
+  Local Notation "'CSUBST' c" := (ctx_subst (typ:=typ) (expr:=expr) c) (at level 0).
 
   (** StateT subst Option Goal **)
   Inductive Result c :=
   | Fail
-  | More_  : ctx_subst c -> Goal -> Result c
-  | Solved : ctx_subst c -> Result c.
+  | More_  : CSUBST c -> Goal -> Result c
+  | Solved : CSUBST c -> Result c.
 
-  Definition More {c} (s : ctx_subst c) (g : Goal) : Result c :=
+  Definition More {c} (s : CSUBST c) (g : Goal) : Result c :=
     match g with
       | GSolved => Solved s
       | _ => More_ s g
@@ -521,7 +151,7 @@ Section parameterized.
   (** Treat this as opaque! **)
   Definition rtac : Type :=
     tenv typ -> tenv typ -> nat -> nat ->
-    forall c : Ctx, ctx_subst c -> expr -> Result c.
+    forall c : Ctx typ expr, ctx_subst c -> expr -> Result c.
 
   Definition propD := @exprD'_typ0 _ _ _ _ Prop _.
 
@@ -559,6 +189,7 @@ Section parameterized.
        | eq_refl => hlist_nth h (length a)
      end).
 
+(*
   Fixpoint goal_substD (tus tvs : list typ)
            (ts : list typ) (es : list (option expr))
   : option (exprT (tus ++ ts) tvs Prop) :=
@@ -588,6 +219,7 @@ Section parameterized.
       | nil , _ :: _ => None
       | _ :: _ , nil => None
     end.
+*)
 
   (** NOTE:
    ** Appending the newly introduced terms makes tactics non-local.
@@ -604,10 +236,10 @@ Section parameterized.
           | Some D =>
             Some (fun us vs => _foralls typD (tv :: nil) (fun vs' => D us (HList.hlist_app vs vs')))
         end
-      | GExs tes goal' =>
-        let tus_ext := map fst tes in
-        match goalD (tus ++ tus_ext) tvs goal'
-            , goal_substD tus tvs tus_ext (map snd tes) with
+      | GExs ts sub goal' =>
+        let tus_ext := ts in
+        match goalD (tus ++ ts) tvs goal'
+            , FMapSubst.SUBST.raw_substD (tus ++ ts) tvs sub with
           | None , _ => None
           | Some _ , None => None
           | Some D , Some sD =>
@@ -651,69 +283,6 @@ Section parameterized.
     clear. destruct pfu; destruct pfv. reflexivity.
   Qed.
 
-  Fixpoint pctxD (tus tvs : tenv typ) (ctx : Ctx) (s : ctx_subst ctx) {struct s}
-  : option (   exprT (tus ++ getUVars ctx) (tvs ++ getVars ctx) Prop
-            -> exprT tus tvs Prop) :=
-    match s in ctx_subst ctx
-          return option (   exprT (tus ++ getUVars ctx) (tvs ++ getVars ctx) Prop
-                         -> exprT tus tvs Prop)
-    with
-      | TopSubst s =>
-        match substD tus tvs s with
-          | None => None
-          | Some sD =>
-            Some (fun (k : exprT _ _ Prop) us vs =>
-                    sD us vs ->
-                    k (hlist_app us Hnil) (hlist_app vs Hnil))
-        end
-      | AllSubst t ctx' s' =>
-        match pctxD tus tvs s' with
-          | Some cD =>
-            Some (fun k : exprT _ _ Prop =>
-                    cD (fun us vs =>
-                          forall x : typD t,
-                            k us
-                              match
-                                app_ass_trans tvs (getVars ctx') (t :: nil) in (_ = t0)
-                                return (hlist typD t0)
-                              with
-                                | eq_refl => hlist_app vs (Hcons x Hnil)
-                              end))
-          | None => None
-        end
-      | ExsSubst ts ctx' s' sub =>
-        match substD ((tus ++ getUVars ctx') ++ ts) (tvs ++ getVars ctx') sub
-            , pctxD tus tvs s'
-        with
-          | Some sD , Some cD =>
-            Some (fun k : exprT (tus ++ getUVars ctx' ++ ts) (tvs ++ getVars ctx') Prop =>
-                    cD (fun us vs =>
-                          _foralls typD ts (fun us' =>
-                                             sD (hlist_app us us') vs ->
-                                             k match
-                                                 app_ass_trans tus _ ts in (_ = t0)
-                                                 return (hlist typD t0)
-                                               with
-                                                 | eq_refl => hlist_app us us'
-                                               end
-                                               vs)))
-          | _ , _ => None
-        end
-      | HypSubst h ctx' s' =>
-        match propD (tus ++ getUVars ctx') (tvs ++ getVars ctx') h with
-          | None => None
-          | Some pD => match pctxD tus tvs s' with
-                         | None => None
-                         | Some cD =>
-                           Some (fun k : exprT _ _ Prop =>
-                                   cD (fun us vs => pD us vs -> k us vs))
-                       end
-        end
-    end.
-
-  Definition RCtx {tus tvs tus' tvs'} :=
-    (RexprT tus tvs Basics.impl ==> RexprT tus' tvs' Basics.impl)%signature.
-
   Local Existing Instance Transitive_Roption.
   Local Existing Instance Symmetric_Roption.
   Local Existing Instance Reflexive_Roption.
@@ -723,21 +292,23 @@ Section parameterized.
 
   Definition EqGoal tus tvs : relation Goal :=
     fun g1 g2 =>
-        Roption (RexprT tus tvs iff)
-                (goalD tus tvs g1)
-                (goalD tus tvs g2).
+      (WellFormed_Goal tus tvs g1 <-> WellFormed_Goal tus tvs g2) /\
+      Roption (RexprT tus tvs iff)
+              (goalD tus tvs g1)
+              (goalD tus tvs g2).
 
   Global Instance Reflexive_EqGoal tus tvs : Reflexive (EqGoal tus tvs).
-  Proof. red. red. reflexivity. Qed.
+  Proof. red. red. split; reflexivity. Qed.
   Global Instance Transitive_EqGoal tus tvs : Transitive (EqGoal tus tvs).
   Proof.
     red. unfold EqGoal. intros.
+    intuition.
     etransitivity; eauto.
   Qed.
   Global Instance Symmetric_EqGoal tus tvs : Symmetric (EqGoal tus tvs).
   Proof.
     red; unfold EqGoal. intros.
-    symmetry. eauto.
+    intuition.
   Qed.
 
   Definition EqResult tus tvs c : relation (Result c) :=
@@ -764,99 +335,14 @@ Section parameterized.
     etransitivity; eauto.
   Qed.
 
-  Theorem Proper_pctxD_iff
-  : forall tus tvs c1 s,
-      Proper (Roption (RexprT (tus ++ getUVars c1) (tvs ++ getVars c1) iff ==>
-                              (RexprT tus tvs iff)))%signature
-             (@pctxD tus tvs c1 s).
-  Proof.
-    induction s; simpl; intros.
-    { destruct (substD tus tvs s); try constructor.
-      do 6 red; intros.
-      apply equiv_eq_eq in H0; subst.
-      apply equiv_eq_eq in H1; subst.
-      eapply impl_iff; try reflexivity.
-      intro. eapply H; reflexivity. }
-    { red; simpl.
-      destruct (pctxD tus tvs s); try constructor.
-      inv_all.
-      do 6 red. intros.
-      eapply IHs; eauto.
-      do 5 red; intros.
-      eapply forall_iff. intros.
-      eapply H; eauto.
-      equivs. reflexivity. }
-    { repeat match goal with
-               | |- context [ match ?X with _ => _ end ] => destruct X ; try constructor
-             end.
-      red; intros.
-      inv_all. eapply IHs.
-      do 5 red; intros.
-      apply equiv_eq_eq in H0.
-      apply equiv_eq_eq in H1. subst.
-      eapply impl_iff. reflexivity.
-      intro. eapply H; reflexivity. }
-    { repeat match goal with
-               | |- context [ match ?X with _ => _ end ] => destruct X ; try solve [ constructor ]
-             end.
-      constructor.
-      inv_all; do 6 red; intros.
-      equivs.
-      eapply IHs; try reflexivity.
-      do 5 red; intros; equivs.
-      eapply _forall_iff. intros.
-      eapply impl_iff. reflexivity.
-      intro. eapply H; reflexivity. }
-  Qed.
-
-  Theorem Proper_pctxD_impl
-  : forall tus tvs c1 s,
-      Proper (Roption (RexprT (tus ++ getUVars c1) (tvs ++ getVars c1) Basics.impl ==>
-                              (RexprT tus tvs Basics.impl)))%signature
-             (@pctxD tus tvs c1 s).
-  Proof.
-    induction s; simpl; intros.
-    { destruct (substD tus tvs s); try constructor.
-      do 7 red; intros.
-      equivs.
-      eapply H; eauto; reflexivity. }
-    { red; simpl.
-      destruct (pctxD tus tvs s); try constructor.
-      inv_all.
-      do 7 red. intros.
-      eapply IHs; eauto.
-      do 6 red; intros.
-      equivs.
-      eapply H; eauto; reflexivity. }
-    { repeat match goal with
-               | |- context [ match ?X with _ => _ end ] => destruct X ; try constructor
-             end.
-      red; intros.
-      inv_all. eapply IHs.
-      do 6 red; intros.
-      equivs.
-      eapply H; eauto; reflexivity. }
-    { repeat match goal with
-               | |- context [ match ?X with _ => _ end ] => destruct X ; try solve [ constructor ]
-             end.
-      constructor.
-      inv_all.
-      do 7 red; intros.
-      eapply IHs; eauto.
-      do 6 red; intros.
-      equivs.
-      eapply _forall_sem; intro.
-      eapply _forall_sem with (x := x0) in H5.
-      intros. eapply H; eauto; reflexivity. }
-  Qed.
-
   Lemma More_More_ tus tvs c s :
     (EqGoal tus tvs ==> @EqResult tus tvs c)%signature
                                             (@More c s) (@More_ c s).
   Proof.
     red. red.
     simpl. intros; subst.
-    destruct x; simpl; repeat constructor; assumption.
+    destruct x; simpl;
+    try solve [ repeat (constructor; try assumption) ].
   Qed.
 
   Inductive GConj_rel : Goal -> Goal -> Goal -> Prop :=
@@ -870,7 +356,11 @@ Section parameterized.
       (EqGoal tus tvs)%signature (GConj_ g1 g2) g.
   Proof.
     clear. inversion 1; subst; red; simpl.
-    - destruct (goalD tus tvs g); constructor.
+    - split.
+      { split; intro.
+        + inversion H0. assumption.
+        + constructor. constructor. assumption. }
+      destruct (goalD tus tvs g); constructor.
       do 5 red; intros.
       rewrite and_comm. rewrite and_true_iff.
       apply equiv_eq_eq in H0; apply equiv_eq_eq in H1; subst; reflexivity.
@@ -890,174 +380,57 @@ Section parameterized.
     (EqGoal tus tvs ==> EqGoal tus tvs ==> EqGoal tus tvs)%signature
                                                           GConj GConj_.
   Proof.
-    unfold EqGoal, respectful; simpl.
+    unfold respectful; simpl.
     intros.
     etransitivity.
     - symmetry. eapply GConj_rel_sound. eapply (GConj_GConj_rel x x0).
     - simpl. inversion H; try reflexivity.
       inversion H0; try reflexivity.
-      constructor.
+      split.
+      { split; inversion 1; constructor; subst; tauto. }
+      simpl.
+      destruct (goalD tus tvs x); destruct (goalD tus tvs x0);
+      inversion H2; inversion H4; subst; constructor.
       do 5 red.
-      intros. eapply and_iff. eapply H3; eauto.
-      intro; eapply H6; eauto.
+      intros. eapply and_iff. eapply H7; auto. intro.
+      eapply H10; eauto.
   Qed.
 
-  Theorem Applicative_pctxD
-  : forall tus tvs ctx s C,
-      @pctxD tus tvs ctx s = Some C ->
-      (forall us vs (P Q : exprT _ _ Prop),
-         C (fun a b => P a b -> Q a b) us vs ->
-         C P us vs ->
-         C Q us vs) /\
-      (forall us vs (Q : exprT _ _ Prop), (forall a b, Q a b) -> C Q us vs).
-  Proof.
-    clear. induction s; simpl; intros.
-    { forward; inv_all; subst.
-      forward_reason; split; eauto. }
-    { forward; inv_all; subst.
-      destruct (IHs _ eq_refl) as [ Hap Hpure ]; clear IHs.
-      generalize (Proper_pctxD_impl tus tvs s).
-      Cases.rewrite_all_goal.
-      intros; inv_all.
-      split.
-      { intros us vs P Q f.
-        eapply Hap.
-        eapply H0; [ | reflexivity | reflexivity | eapply f ].
-        simpl. clear.
-        do 6 red. intros; equivs; eauto. }
-      { intros us vs Q v.
-        eapply Hpure. intros; eauto. } }
-    { forward; inv_all; subst.
-      destruct (IHs _ eq_refl) as [ Hap Hpure ]; clear IHs.
-      generalize (Proper_pctxD_impl tus tvs s).
-      Cases.rewrite_all_goal; intros; inv_all.
-      split.
-      { intros us vs P Q f.
-        eapply Hap.
-        eapply H1; [ | reflexivity | reflexivity | eapply f ].
-        clear.
-        do 6 red; intros; equivs.
-        tauto. }
-      { intros. eapply Hpure.
-        intros. eauto. } }
-    { forward; inv_all; subst.
-      destruct (IHs _ eq_refl) as [ Hap Hpure ]; clear IHs.
-      generalize (Proper_pctxD_impl tus tvs s).
-      Cases.rewrite_all_goal.
-      intros; inv_all.
-      split.
-      { intros us vs P Q f.
-        eapply Hap.
-        eapply H1; [ | reflexivity | reflexivity | eapply f ].
-        simpl. clear.
-        do 6 red. intros; equivs; eauto.
-        eapply _forall_sem. intros.
-        rewrite _forall_sem in H2.
-        rewrite _forall_sem in H1.
-        eauto. }
-      { intros us vs Q v.
-        eapply Hpure. intros.
-        eapply _forall_sem; intros.
-        eauto. } }
-  Qed.
-
-  Lemma Ap_pctxD
-  : forall tus tvs (ctx : Ctx) (s : ctx_subst ctx)
-           (C : exprT (tus ++ getUVars ctx) (tvs ++ getVars ctx) Prop ->
-                exprT tus tvs Prop),
-      pctxD tus tvs s = Some C ->
-      forall (us : hlist typD tus) (vs : hlist typD tvs)
-             (P Q : exprT (tus ++ getUVars ctx) (tvs ++ getVars ctx) Prop),
-        C (fun us vs => P us vs -> Q us vs) us vs -> C P us vs -> C Q us vs.
-  Proof.
-    intros. revert H1. revert H0. eapply Applicative_pctxD in H; eauto.
-    destruct H. eapply H.
-  Qed.
-
-  Lemma Pure_pctxD
-  : forall tus tvs (ctx : Ctx) (s : ctx_subst ctx)
-           (C : exprT (tus ++ getUVars ctx) (tvs ++ getVars ctx) Prop ->
-                exprT tus tvs Prop),
-      pctxD tus tvs s = Some C ->
-      forall (P : exprT (tus ++ getUVars ctx) (tvs ++ getVars ctx) Prop),
-        (forall us vs, P us vs) -> forall us vs, C P us vs.
-  Proof.
-    intros. eapply Applicative_pctxD in H; eauto.
-    destruct H. eapply H1; eauto.
-  Qed.
-
-  Definition CtxMorphism {tus tvs tus' tvs'}
-             (c1 c2 : exprT tus tvs Prop -> exprT tus' tvs' Prop) : Prop :=
-    forall (P : exprT _ _ Prop) us vs, c1 P us vs -> c2 P us vs.
-
-  Inductive SubstMorphism (tus tvs : tenv typ)
-  : forall c : Ctx, ctx_subst c -> ctx_subst c -> Prop :=
-  | SMall : forall c t s1 s2,
-              @SubstMorphism tus tvs c s1 s2 ->
-              @SubstMorphism tus tvs (CAll c t) (AllSubst s1) (AllSubst s2)
-  | SMexs : forall c ts s1 s2 cs1 cs2,
-              (match @pctxD tus tvs c cs1
-                   , substD ((tus ++ getUVars c) ++ ts) (tvs ++ getVars c) s1
-                   , @pctxD tus tvs c cs2
-                   , substD ((tus ++ getUVars c) ++ ts) (tvs ++ getVars c) s2
-               with
-                 | None , _ , _ , _
-                 | Some _ , None , _ , _ => True
-                 | Some _ , Some _ , None , _
-                 | Some _ , Some _ , Some _ , None => False
-                 | Some c1D , Some s1D , Some c2D , Some s2D =>
-                   forall us vs, c2D (fun us vs =>
-                                       forall us',
-                                         s2D (hlist_app us us') vs ->
-                                         s1D (hlist_app us us') vs) us vs
-               end) ->
-              @SubstMorphism tus tvs c cs1 cs2 ->
-              @SubstMorphism tus tvs (CExs c ts) (ExsSubst cs1 s1) (ExsSubst cs2 s2)
-  | SMhyp : forall c h s1 s2,
-              @SubstMorphism tus tvs c s1 s2 ->
-              @SubstMorphism tus tvs (CHyp c h) (HypSubst s1) (HypSubst s2)
-  | SMtop : forall s1 s2,
-              match substD tus tvs s1
-                  , substD tus tvs s2
-              with
-                | None , _ => True
-                | Some _ , None => False
-                | Some a , Some b => forall us vs, b us vs -> a us vs
-              end ->
-              @SubstMorphism tus tvs CTop (TopSubst s1) (TopSubst s2).
-
-  Definition rtac_spec tus tvs ctx s g r : Prop :=
+  Definition rtac_spec tus tvs ctx (s : CSUBST ctx) g r : Prop :=
     match r with
       | Fail => True
       | Solved s' =>
+        WellFormed_Goal (tus ++ getUVars ctx) (tvs ++ getVars ctx) g ->
         WellFormed_ctx_subst s ->
         WellFormed_ctx_subst s' /\
-        match @pctxD tus tvs ctx s
-            , goalD _ _ g
-            , @pctxD tus tvs ctx s'
+        match pctxD tus tvs s
+            , goalD (tus ++ getUVars ctx) (tvs ++ getVars ctx) g
+            , pctxD tus tvs s'
         with
           | None , _ , _
           | Some _ , None , _ => True
           | Some _ , Some _ , None => False
           | Some cD , Some gD , Some cD' =>
-            @SubstMorphism tus tvs ctx s s' /\
+            SubstMorphism tus tvs s s' /\
             forall us vs,
               cD' gD us vs
         end
       | More_ s' g' =>
+        WellFormed_Goal (tus ++ getUVars ctx) (tvs ++ getVars ctx) g ->
         WellFormed_ctx_subst s ->
         WellFormed_ctx_subst s' /\
-        match @pctxD tus tvs ctx s
-            , goalD _ _ g
-            , @pctxD tus tvs ctx s'
-            , goalD _ _ g'
+        WellFormed_Goal (tus ++ getUVars ctx) (tvs ++ getVars ctx) g' /\
+        match pctxD tus tvs s
+            , goalD (tus ++ getUVars ctx) (tvs ++ getVars ctx) g
+            , pctxD tus tvs s'
+            , goalD (tus ++ getUVars ctx) (tvs ++ getVars ctx) g'
         with
           | None , _ , _ , _
           | Some _ , None , _ , _ => True
           | Some _ , Some _ , None , _
           | Some _ , Some _ , Some _ , None => False
           | Some cD , Some gD , Some cD' , Some gD' =>
-            @SubstMorphism tus tvs ctx s s' /\
+            SubstMorphism tus tvs s s' /\
             forall us vs, cD' (fun us vs => gD' us vs -> gD us vs) us vs
         end
     end.
@@ -1069,25 +442,15 @@ Section parameterized.
        tac tus tvs (length tus) (length tvs) ctx s g = result) ->
       @rtac_spec tus tvs ctx s (GGoal g) result.
 
-  Lemma Fmap_pctxD_impl
-  : forall tus tvs c s C,
-      @pctxD tus tvs c s = Some C ->
-      Proper (RexprT _ _ Basics.impl ==> RexprT tus tvs Basics.impl)%signature C.
-  Proof.
-    clear. intros.
-    generalize (@Proper_pctxD_impl tus tvs c s).
-    rewrite H. intros; inv_all. auto.
-  Qed.
+  Lemma left_side : forall (P Q R : Prop), P ->
+                                           (Q <-> R) ->
+                                           ((P /\ Q) <-> R).
+  Proof. tauto. Qed.
 
-  Lemma Fmap_pctxD_iff
-  : forall tus tvs c s C,
-      @pctxD tus tvs c s = Some C ->
-      Proper (RexprT _ _ iff ==> RexprT tus tvs iff)%signature C.
-  Proof.
-    clear. intros.
-    generalize (@Proper_pctxD_iff tus tvs c s).
-    rewrite H. intros; inv_all. auto.
-  Qed.
+  Lemma right_side : forall (P Q R : Prop), P ->
+                                           (Q <-> R) ->
+                                           (Q <-> (P /\ R)).
+  Proof. tauto. Qed.
 
 
   Theorem Proper_rtac_spec tus tvs ctx s
@@ -1101,275 +464,46 @@ Section parameterized.
       reflexivity. }
     { destruct x0; destruct y0; simpl in *;
       try solve [ reflexivity | congruence ]; inv_all; subst; inv_all;
-      try (eapply impl_iff; try reflexivity; intros;
-           eapply and_iff; try reflexivity; intros;
-           try inversion H; try reflexivity;
-           try inversion H5; try reflexivity;
-           repeat match goal with
-                    | |- context [ match ?X with _ => _ end ] =>
-                      consider X; intros; try reflexivity; [ ]
-                  end;
-           eapply and_iff; try reflexivity; intros;
-           do 2 (eapply forall_iff; intro);
-           eapply Fmap_pctxD_iff; eauto; try reflexivity;
-           do 5 red; intros).
-      { apply impl_iff; [ eapply H10; eauto | intro ].
-        apply H7; eauto. }
-      { do 5 red in H10.
-        rewrite H10; try reflexivity.
+      repeat match goal with
+               | H : ?X , H' : ?X |- _ => clear H'
+               | H : EqGoal _ _ _ _ |- _ => destruct H
+               | |- (_ -> _) <-> (_ -> _) =>
+                 eapply impl_iff; [ solve [ eauto | reflexivity ] | ]; intros
+               | |- (_ /\ _) <-> (_ /\ _) =>
+                 eapply and_iff; [ solve [ eauto | reflexivity ] | ]; intros
+               | H : Roption _ _ _ |- _ => inversion H; clear H
+               | |- context [ match ?X with _ => _ end ] =>
+                 consider X; intros; try reflexivity; [ ]
+               | |- context [ match ?X with _ => _ end ] =>
+                 consider X; intros; reflexivity
+               | |- (forall x, _) <-> (forall y, _) =>
+                 eapply forall_iff; intro
+               | |- _ =>
+                 eapply left_side; [ match goal with
+                                       | H : _ <-> _ |- _ => apply H; constructor
+                                     end | ]
+               | |- _ =>
+                 eapply right_side; [ match goal with
+                                       | H : _ <-> _ |- _ => apply H; constructor
+                                     end | ]
+             end.
+      { eapply Fmap_pctxD_iff; eauto; try reflexivity.
+        do 5 red; intros.
+        apply impl_iff; [ eapply H10; eauto | intro ].
+        apply H12; eauto. }
+      { eapply Fmap_pctxD_iff; eauto; try reflexivity.
+        do 5 red; intros.
+        do 5 red in H9. subst.
+        rewrite H9; eauto.
         rewrite impl_True_iff.
-        eapply H7; eauto. }
-      { do 5 red in H10.
-        rewrite <- H10; try reflexivity.
+        eapply H11; eauto. }
+      { eapply Fmap_pctxD_iff; eauto; try reflexivity.
+        do 5 red; intros.
+        do 5 red in H9. subst.
+        rewrite <- H9; eauto.
         rewrite impl_True_iff.
-        eapply H7; eauto. } }
-  Qed.
-
-  Lemma pctxD_SubstMorphism
-  : forall tus tvs ctx s s',
-      @SubstMorphism tus tvs ctx s s' ->
-      forall C C',
-      @pctxD tus tvs ctx s = Some C ->
-      @pctxD tus tvs ctx s' = Some C' ->
-      forall us vs (P : exprT _ _ Prop),
-        C P us vs -> C' P us vs.
-  Proof.
-    induction 1; intros; simpl in *; forward; inv_all; subst; eauto.
-    { eapply IHSubstMorphism; eauto. }
-    { simpl in *.
-      eapply (IHSubstMorphism _ _ eq_refl eq_refl) in H3.
-      destruct (Applicative_pctxD _ H2) as [ Hap Hpure ].
-      revert H3. eapply Hap.
-      generalize (H7 us vs).
-      eapply Hap.
-      eapply Hpure.
-      clear. intros.
-      rewrite _forall_sem.
-      rewrite _forall_sem in H0.
-      intros; eauto. }
-    { eapply IHSubstMorphism; eauto. }
-  Qed.
-
-  Definition fromTop (cs : ctx_subst CTop) : subst :=
-    match cs in ctx_subst c
-          return match c with
-                   | CTop => subst
-                   | _ => unit
-                 end
-    with
-      | TopSubst c => c
-      | _ => tt
-    end.
-
-  Definition fromAll {c t} (cs : ctx_subst (CAll c t)) : ctx_subst c :=
-    match cs in ctx_subst c
-          return match c with
-                   | CAll c _ => ctx_subst c
-                   | _ => unit
-                 end
-    with
-      | AllSubst _ _ c => c
-      | _ => tt
-    end.
-
-  Definition fromHyp {c t} (cs : ctx_subst (CHyp c t)) : ctx_subst c :=
-    match cs in ctx_subst c
-          return match c with
-                   | CHyp c _ => ctx_subst c
-                   | _ => unit
-                 end
-    with
-      | HypSubst _ _ c => c
-      | _ => tt
-    end.
-
-  Definition fromExs {c t} (cs : ctx_subst (CExs c t)) : subst * ctx_subst c :=
-    match cs in ctx_subst c
-          return match c with
-                   | CExs c _ => subst * ctx_subst c
-                   | _ => unit
-                 end
-    with
-      | ExsSubst _ _ c s => (s,c)
-      | _ => tt
-    end.
-
-  Global Instance Injective_SubstMorphism_AllSubst tus tvs t ctx s s'
-  : Injective (@SubstMorphism tus tvs (CAll ctx t) (AllSubst s) s') :=
-  { result := exists s'', s' = AllSubst s'' /\ @SubstMorphism tus tvs ctx s s'' }.
-  intros.
-  exists (fromAll s').
-  refine
-    (match H in @SubstMorphism _ _ C X Y
-           return match X in ctx_subst C' return ctx_subst C' -> Prop with
-                    | AllSubst t s c => fun s' =>
-                                            s' = AllSubst (fromAll s') /\
-                                            SubstMorphism tus tvs c (fromAll s')
-                    | _ => fun _ => True
-                  end Y
-     with
-       | SMall _ _ _ _ _ => _
-       | _ => I
-     end).
-  simpl; eauto.
-  Defined.
-
-  Global Instance Injective_SubstMorphism_HypSubst tus tvs t ctx s s'
-  : Injective (@SubstMorphism tus tvs (CHyp ctx t) (HypSubst s) s') :=
-  { result := exists s'', s' = HypSubst s'' /\ @SubstMorphism tus tvs ctx s s'' }.
-  intros.
-  exists (fromHyp s').
-  refine
-    (match H in @SubstMorphism _ _ C X Y
-           return match X in ctx_subst C' return ctx_subst C' -> Prop with
-                    | HypSubst t s c => fun s' =>
-                                            s' = HypSubst (fromHyp s') /\
-                                            SubstMorphism tus tvs c (fromHyp s')
-                    | _ => fun _ => True
-                  end Y
-     with
-       | SMhyp _ _ _ _ _ => _
-       | _ => I
-     end).
-  simpl; eauto.
-  Defined.
-
-  Global Instance Injective_SubstMorphism_TopSubst tus tvs s s'
-  : Injective (@SubstMorphism tus tvs (CTop) (TopSubst s) s') :=
-  { result := exists s'', s' = TopSubst s'' /\ match substD tus tvs s
-                                                   , substD tus tvs s''
-                                               with
-                                                 | None , _ => True
-                                                 | Some _ , None => False
-                                                 | Some a , Some b => forall us vs, b us vs -> a us vs
-                                               end }.
-  Proof.
-    intros.
-    exists (fromTop s').
-    refine
-      (match H in @SubstMorphism _ _ C X Y
-             return match X in ctx_subst C' return ctx_subst C' -> Prop with
-                      | TopSubst s => fun s' =>
-                                        s' = TopSubst (fromTop s') /\
-                                        match substD tus tvs s
-                                            , substD tus tvs (fromTop s')
-                                        with
-                                          | None , _ => True
-                                          | Some _ , None => False
-                                          | Some a , Some b => forall us vs, b us vs -> a us vs
-                                        end
-                      | _ => fun _ => True
-                    end Y
-       with
-         | SMtop _ _ _ => _
-         | _ => I
-       end).
-    simpl; eauto.
-  Defined.
-
-  Global Instance Injective_SubstMorphism_ExsSubst tus tvs ctx tes s s' sub
-  : Injective (@SubstMorphism tus tvs (CExs ctx tes) (ExsSubst sub s) s') :=
-  { result := exists s'' sub',
-                s' = ExsSubst sub' s''
-                /\ (match @pctxD tus tvs ctx sub
-                        , substD ((tus ++ getUVars ctx) ++ tes) (tvs ++ getVars ctx) s
-                        , @pctxD tus tvs ctx sub'
-                        , substD ((tus ++ getUVars ctx) ++ tes) (tvs ++ getVars ctx) s''
-                    with
-                      | None , _ , _ , _
-                      | Some _ , None , _ , _ => True
-                      | Some _ , Some _ , None , _
-                      | Some _ , Some _ , Some _ , None => False
-                      | Some c1D , Some s1D , Some c2D , Some s2D =>
-                        forall us vs, c2D (fun us vs =>
-                                             forall us',
-                                               s2D (hlist_app us us') vs ->
-                                               s1D (hlist_app us us') vs) us vs
-                    end)
-                /\ SubstMorphism tus tvs sub sub'}.
-  intros. exists (fst (fromExs s')). exists (snd (fromExs s')).
-  refine
-    (match H in @SubstMorphism _ _ C X Y
-           return match X in ctx_subst C' return ctx_subst C' -> Prop with
-                    | ExsSubst t s su c =>
-                      fun s' =>
-                        s' = ExsSubst (snd (fromExs s')) (fst (fromExs s')) /\
-                        match pctxD tus tvs su with
-                          | Some _ =>
-                            match
-                              substD ((tus ++ getUVars s) ++ t) (tvs ++ getVars s) c
-                            with
-                              | Some s1D =>
-                                match pctxD tus tvs (snd (fromExs s')) with
-                                  | Some c2D =>
-                                    match
-                                      substD ((tus ++ getUVars s) ++ t)
-                                             (tvs ++ getVars s) (fst (fromExs s'))
-                                    with
-                                      | Some s2D =>
-                                        forall us vs,
-                                          c2D
-                                            (fun us0 vs0 =>
-                                               forall us' : hlist typD t,
-                                                 s2D (hlist_app us0 us') vs0 ->
-                                                 s1D (hlist_app us0 us') vs0) us vs
-                                      | None => False
-                                    end
-                                  | None => False
-                                end
-                              | None => True
-                            end
-                          | None => True
-                        end /\
-                        SubstMorphism tus tvs su (snd (fromExs s'))
-                    | _ => fun _ => True
-                  end Y
-     with
-       | SMexs _ _ _ _ _ _ _ _ => _
-       | _ => I
-     end).
-  simpl; eauto.
-  Defined.
-
-  Global Instance Reflexive_SubstMorphism tus tvs ctx
-  : Reflexive (@SubstMorphism tus tvs ctx).
-  Proof.
-    red. induction x;
-         simpl; intros; try constructor;
-         forward; eauto.
-    eapply Applicative_pctxD; eauto.
-  Qed.
-
-  Global Instance Transitive_SubstMorphism tus tvs ctx
-  : Transitive (@SubstMorphism tus tvs ctx).
-  Proof.
-    clear. red. intros x y z H; revert z.
-    induction H.
-    { intros; inv_all; subst.
-      constructor; eauto. }
-    { intros; inv_all; subst.
-      forward. simpl in *.
-      constructor.
-      { forward. inv_all; subst.
-        Cases.rewrite_all_goal.
-        repeat match goal with
-                 | H : ?X = _ , H' : ?X = _ |- _ =>
-                   rewrite H in H'
-               end; inv_all; subst.
-        specialize (H8 us vs).
-        specialize (H6 us vs).
-        revert H8.
-        eapply (Applicative_pctxD _ H5).
-        eapply (pctxD_SubstMorphism H4 H1 H5 us vs).
-        revert H6.
-        eapply (Fmap_pctxD_impl _ H1); try reflexivity.
-        clear.
-        do 6 red. intros. equivs. firstorder. }
-      { eapply IHSubstMorphism. eassumption. } }
-    { intros; inv_all; subst. constructor; eauto. }
-    { intros; inv_all; subst.
-      constructor.
-      forward. eauto. }
+        eapply H11; eauto. }
+      { eapply Fmap_pctxD_iff; eauto; try reflexivity. } }
   Qed.
 
   Theorem rtac_spec_More_
@@ -1380,6 +514,7 @@ Section parameterized.
     intros; subst.
     split; auto.
     simpl. forward.
+    split; auto.
     split; try reflexivity.
     intros. eapply Applicative_pctxD; eauto.
   Qed.
@@ -1399,24 +534,21 @@ Section parameterized.
   Proof.
     destruct r; simpl; intros; auto; forward; forward_reason;
     split; eauto.
-    - split; [ etransitivity; eauto | ].
-      intros us vs. generalize (H11 us vs); clear H11.
-      destruct (Applicative_pctxD _ H4) as [ Hap Hpure ].
-      eapply Hap.
-      eapply (pctxD_SubstMorphism H10 H0 H4).
-      generalize (H9 us vs); clear H9.
-      clear Hap Hpure.
+    - split; auto.
+      split; [ eapply Transitive_SubstMorphism; eauto | ].
+      intros us vs. generalize (H14 us vs); clear H14.
+      eapply Ap_pctxD; eauto.
+      eapply pctxD_SubstMorphism; eauto.
+      generalize (H11 us vs); clear H11.
       eapply Fmap_pctxD_impl;
         [ eassumption | | reflexivity | reflexivity ].
       clear. do 6 red.
       intros; equivs. tauto.
-    - split; [ etransitivity; eauto | ].
-      intros us vs. generalize (H10 us vs); clear H10.
-      destruct (Applicative_pctxD _ H4) as [ Hap Hpure ].
-      eapply Hap.
-      eapply (pctxD_SubstMorphism H9 H0 H4).
-      generalize (H8 us vs); clear H8.
-      clear Hap Hpure.
+    - split; [ eapply Transitive_SubstMorphism; eauto | ].
+      intros us vs. generalize (H12 us vs); clear H12.
+      eapply Ap_pctxD; eauto.
+      eapply pctxD_SubstMorphism; eauto.
+      generalize (H10 us vs); clear H10.
       eapply Fmap_pctxD_impl;
         [ eassumption | | reflexivity | reflexivity ].
       clear. do 6 red.
@@ -1425,9 +557,9 @@ Section parameterized.
 
 End parameterized.
 
-Arguments rtac_sound {typ expr subst _ _ _ _ _} tus tvs tac : rename.
+Arguments rtac_sound {typ expr _ _ _} tus tvs tac : rename.
 
-Arguments GEx {typ expr} _ _ _ : rename.
+(*Arguments GEx {typ expr} _ _ _ : rename. *)
 Arguments GAll {typ expr} _ _ : rename.
 Arguments GHyp {typ expr} _ _ : rename.
 Arguments GConj {typ expr} _ _ : rename.
@@ -1435,16 +567,13 @@ Arguments GConj_ {typ expr} _ _ : rename.
 Arguments GConj_list {typ expr} _ : rename.
 Arguments GGoal {typ expr} _ : rename.
 Arguments GSolved {typ expr} : rename.
-Arguments CTop {typ expr} : rename.
-Arguments CEx {typ expr} _ _ : rename.
-Arguments CAll {typ expr} _ _ : rename.
-Arguments CHyp {typ expr} _ _ : rename.
 
-Arguments Fail {typ expr subst _} : rename.
-Arguments More {typ expr subst _} _ _ : rename.
-Arguments More_ {typ expr subst _} _ _ : rename.
-Arguments Solved {typ expr subst _} _ : rename.
+Arguments Fail {typ expr _} : rename.
+Arguments More {typ expr _} _ _ : rename.
+Arguments More_ {typ expr _} _ _ : rename.
+Arguments Solved {typ expr _} _ : rename.
 
 Export MirrorCore.ExprI.
 Export MirrorCore.SubstI.
 Export MirrorCore.ExprDAs.
+Export MirrorCore.RTac.Ctx.
