theories/RTac/Ctx.v
@@ -1,0 +1,958 @@
+Require Import Coq.Classes.Morphisms.
+Require Import Coq.Relations.Relations.
+Require Import ExtLib.Core.RelDec.
+Require Import ExtLib.Structures.Monad.
+Require Import ExtLib.Structures.Traversable.
+Require Import ExtLib.Data.Option.
+Require Import ExtLib.Data.Prop.
+Require Import ExtLib.Data.Pair.
+Require Import ExtLib.Data.List.
+Require Import ExtLib.Data.HList.
+Require Import ExtLib.Data.Monads.OptionMonad.
+Require Import ExtLib.Tactics.
+Require Import MirrorCore.ExprI.
+Require Import MirrorCore.SubstI.
+Require Import MirrorCore.ExprDAs.
+
+Require Import MirrorCore.Util.Quant.
+Require Import MirrorCore.Util.Forwardy.
+
+Set Implicit Arguments.
+Set Strict Implicit.
+
+Ltac equivs :=
+  repeat match goal with
+           | H : equiv_hlist _ _ _ |- _ => apply equiv_eq_eq in H
+         end; subst.
+
+Section parameterized.
+  Variable typ : Type.
+  Variable expr : Type.
+
+  Context {RType_typ : RType typ}.
+  Context {Typ0_Prop : Typ0 _ Prop}.
+  Context {Expr_expr : Expr RType_typ expr}.
+  Context {ExprOk_expr : ExprOk Expr_expr}.
+
+  Variable instantiate : (nat -> option expr) -> nat -> expr -> expr.
+
+  Inductive Ctx :=
+  | CTop
+  | CAll : Ctx -> typ -> Ctx
+  | CExs : Ctx -> list typ -> Ctx
+  | CHyp : Ctx -> expr -> Ctx.
+
+  Fixpoint CEx (c : Ctx) (t : typ) : Ctx :=
+    CExs c (t :: nil).
+
+  Fixpoint CAlls (c : Ctx) (ls : list typ) : Ctx :=
+    match ls with
+      | nil => c
+      | l :: ls => CAlls (CAll c l) ls
+    end.
+
+  (** Auxiliary Functions **)
+  Fixpoint countVars (ctx : Ctx) : nat :=
+    match ctx with
+      | CTop => 0
+      | CAll ctx' t => S (countVars ctx')
+      | CExs ctx' _
+      | CHyp ctx' _ => countVars ctx'
+    end.
+
+  Fixpoint countUVars (ctx : Ctx) : nat :=
+    match ctx with
+      | CTop => 0
+      | CExs ctx' ts => length ts + countUVars ctx'
+      | CAll ctx' _
+      | CHyp ctx' _ => countUVars ctx'
+    end.
+
+  Fixpoint getUVars (ctx : Ctx) : tenv typ :=
+    match ctx with
+      | CTop => nil
+      | CAll ctx' _ => getUVars ctx'
+      | CExs ctx' ts => getUVars ctx' ++ ts
+      | CHyp ctx' _ => getUVars ctx'
+    end.
+
+  Fixpoint getVars (ctx : Ctx) : tenv typ :=
+    match ctx with
+      | CTop => nil
+      | CAll ctx' t => getVars ctx' ++ t :: nil
+      | CExs ctx' _ => getVars ctx'
+      | CHyp ctx' _ => getVars ctx'
+    end.
+
+  Lemma countVars_getVars : forall ctx, countVars ctx = length (getVars ctx).
+    induction ctx; simpl; auto.
+    rewrite app_length. simpl. omega.
+  Qed.
+
+  Lemma countUVars_getUVars : forall ctx, countUVars ctx = length (getUVars ctx).
+    induction ctx; simpl; auto.
+    rewrite app_length. simpl. omega.
+  Qed.
+
+  Fixpoint getEnvs' (ctx : Ctx) (tus tvs : tenv typ)
+  : tenv typ * tenv typ :=
+    match ctx with
+      | CTop => (tus,tvs)
+      | CAll ctx' t => getEnvs' ctx' tus (t :: tvs)
+      | CExs ctx' ts => getEnvs' ctx' (ts ++ tus) tvs (** TODO: Check **)
+      | CHyp ctx' _ => getEnvs' ctx' tus tvs
+    end.
+
+  Definition getEnvs (ctx : Ctx) : tenv typ * tenv typ :=
+    let (x,y) := getEnvs' ctx nil nil in
+    (x, y).
+
+  Fixpoint Ctx_append (c1 c2 : Ctx) : Ctx :=
+    match c2 with
+      | CTop => c1
+      | CAll ctx' t => CAll (Ctx_append c1 ctx') t
+      | CExs ctx' ts => CExs (Ctx_append c1 ctx') ts
+      | CHyp ctx' h => CHyp (Ctx_append c1 ctx') h
+    end.
+
+  Theorem getUVars_append
+  : forall c1 c2,
+      getUVars (Ctx_append c1 c2) = getUVars c1 ++ getUVars c2.
+  Proof.
+    clear. induction c2; simpl; eauto.
+    symmetry; eapply app_nil_r_trans.
+    rewrite IHc2. apply app_ass_trans.
+  Defined.
+
+  Theorem getVars_append
+  : forall c1 c2,
+      getVars (Ctx_append c1 c2) = getVars c1 ++ getVars c2.
+  Proof.
+    clear. induction c2; simpl; eauto.
+    symmetry; eapply app_nil_r_trans.
+    rewrite IHc2. apply app_ass_trans.
+  Defined.
+  (** End: Auxiliary Functions **)
+
+  Require Import MirrorCore.Subst.FMapSubst.
+
+  Definition amap : Type := SUBST.raw expr.
+  Definition amap_lookup : nat -> amap -> option expr :=
+    @UVarMap.MAP.find _.
+  Definition amap_check_set : nat -> expr -> amap -> option amap :=
+    @SUBST.raw_set _ _ _ _ instantiate.
+
+  Inductive ctx_subst : Ctx -> Type :=
+  | TopSubst : ctx_subst CTop
+  | AllSubst : forall {t c}, ctx_subst c -> ctx_subst (CAll c t)
+  | HypSubst : forall {t c}, ctx_subst c -> ctx_subst (CHyp c t)
+  | ExsSubst : forall {ts c}, ctx_subst c -> amap -> ctx_subst (CExs c ts).
+
+  Definition only_in_range (min len : nat) (s : amap) : Prop :=
+    forall u e, amap_lookup u s = Some e -> min <= u < min + len.
+
+  (** [tus] and [tvs] are full environments! **)
+  (** TODO: Maybe they should just be the bottom? **)
+  Inductive WellFormed_ctx_subst
+  : forall c, tenv typ -> tenv typ -> ctx_subst c -> Prop :=
+  | WF_TopSubst : forall tus tvs, WellFormed_ctx_subst tus tvs TopSubst
+  | WF_AllSubst : forall tus tvs t c s,
+                    WellFormed_ctx_subst tus tvs s ->
+                    WellFormed_ctx_subst tus (tvs ++ t :: nil) (@AllSubst t c s)
+  | WF_HypSubst : forall tus tvs t c s,
+                    WellFormed_ctx_subst tus tvs s ->
+                    WellFormed_ctx_subst tus tvs (@HypSubst t c s)
+  | WF_ExsSubst : forall tus tvs ts c s s',
+                    SUBST.WellFormed s' ->
+                    only_in_range (length tus + countUVars c) (length ts) s' ->
+                    WellFormed_ctx_subst tus tvs s ->
+                    WellFormed_ctx_subst (tus ++ ts) tvs (@ExsSubst ts c s s').
+
+  Fixpoint ctx_lookup {c} (u : nat) (cs : ctx_subst c) : option expr :=
+    match cs with
+      | TopSubst => None
+      | AllSubst _ _ c => ctx_lookup u c
+      | HypSubst _ _ c => ctx_lookup u c
+      | ExsSubst _ _ c s =>
+        match amap_lookup u s with
+          | None => ctx_lookup u c
+          | Some e => Some e
+        end
+    end.
+
+  Fixpoint ctx_domain {c} (cs : ctx_subst c) : list nat :=
+    match cs with
+      | TopSubst => nil
+      | AllSubst _ _ c => ctx_domain c
+      | HypSubst _ _ c => ctx_domain c
+      | ExsSubst _ _ c s =>
+        ctx_domain c ++ map fst (UVarMap.MAP.elements s)
+    end.
+
+  Fixpoint all_convertible (xs ys : tenv typ) : bool :=
+    match xs , ys with
+      | nil , nil => true
+      | x :: xs , y :: ys =>
+        match type_cast x y with
+          | None => false
+          | Some _ => all_convertible xs ys
+        end
+      | _ , _ => false
+    end.
+
+  Theorem all_convertible_sound
+  : forall xs ys,
+      all_convertible xs ys = true -> xs = ys.
+  Proof.
+    induction xs; destruct ys; simpl; intros; try congruence.
+    destruct (type_cast a t).
+    { destruct r. f_equal; eauto. }
+    { congruence. }
+  Qed.
+
+  Definition drop_exact (tus ts : tenv typ)
+  : option { ts' : tenv typ & hlist typD tus -> hlist typD ts' } :=
+    let rem_len := length tus - length ts in
+    let x := skipn rem_len tus in
+    if all_convertible x ts then
+      Some (@existT _ (fun ts' => hlist typD tus -> hlist typD ts')
+                    (firstn rem_len tus)
+                    (fun x =>
+                       fst (hlist_split
+                              (firstn rem_len tus)
+                              (skipn rem_len tus)
+                              match eq_sym (firstn_skipn _ _) in _ = l
+                                    return hlist _ l with
+                                | eq_refl => x
+                              end)))
+    else
+      None.
+
+  Fixpoint ctx_substD {c} tus tvs (cs : ctx_subst c) {struct cs}
+  : option (exprT tus tvs Prop) :=
+    match cs with
+      | TopSubst => Some (fun _ _ => True)
+      | HypSubst _ _ c => ctx_substD tus tvs c
+      | AllSubst t _ c =>
+        match drop_exact tvs (t :: nil) with
+          | None => None
+          | Some (existT tvs' get) =>
+            match ctx_substD tus tvs' c with
+              | None => None
+              | Some sD => Some (fun us vs => sD us (get vs))
+            end
+        end
+      | ExsSubst ts _ c s =>
+        match drop_exact tus ts with
+          | None => None
+          | Some (existT tus' get) =>
+            match SUBST.raw_substD tus tvs s
+                , ctx_substD tus' tvs c
+            with
+              | Some sD' , Some sD =>
+                Some (fun us vs => sD' us vs /\ sD (get us) vs)
+              | None , _ => None
+              | Some _ , None => None
+            end
+        end
+    end.
+
+  Section ctx_set'.
+    Variables (u : nat) (e : expr) (min : nat) (nus : nat).
+
+    Fixpoint ctx_set' {c T} (cs : ctx_subst c) {struct cs}
+    : ((nat -> option expr) -> ctx_subst c -> option T) -> option T :=
+      match cs in ctx_subst c
+            return ((nat -> option expr) -> ctx_subst c -> option T) -> option T
+      with
+        | TopSubst => fun k => None
+        | AllSubst _ _ c => fun k =>
+          ctx_set' c (fun f c => k f (AllSubst c))
+        | HypSubst _ _ c => fun k =>
+          ctx_set' c (fun f c => k f (HypSubst c))
+        | ExsSubst _ ctx c s => fun k =>
+          if u ?[ ge ] (countUVars ctx + nus) then
+            match amap_check_set u e s with
+              | None => None
+              | Some s' =>
+                match amap_lookup u s with
+                  | None => None
+                  | Some e' =>
+                    k (fun x => if x ?[ eq ] u then Some e' else None)
+                      (ExsSubst c s')
+                end
+            end
+          else
+            ctx_set' c
+                     (fun f c => k f (@ExsSubst _ ctx c
+                                                (SUBST.raw_instantiate instantiate f s)))
+      end.
+  End ctx_set'.
+
+  Definition ctx_set {c} (u : nat) (e : expr) (cs : ctx_subst c)
+  : option (ctx_subst c) :=
+    ctx_set' u e 0 cs (fun _ => @Some _).
+
+  Fixpoint ctx_empty {c} : ctx_subst c :=
+    match c with
+      | CTop => TopSubst
+      | CHyp c h => HypSubst ctx_empty
+      | CAll c h => AllSubst ctx_empty
+      | CExs c h => ExsSubst ctx_empty (UVarMap.MAP.empty _)
+    end.
+
+  Global Instance Subst_ctx_subst ctx : Subst (ctx_subst ctx) expr :=
+  { subst_lookup := ctx_lookup
+  ; subst_domain := ctx_domain
+  }.
+
+  Lemma drop_exact_sound
+  : forall tus ts tus' cast,
+      drop_exact tus ts = Some (@existT _ _ tus' cast) ->
+      exists pf : tus' ++ ts = tus,
+        forall a b, cast match pf in _ = tus return hlist _ tus with
+                           | eq_refl => hlist_app a b
+                         end = a.
+  Proof.
+    clear. unfold drop_exact. intros.
+    forward; inv_all; subst.
+    subst.
+    eapply all_convertible_sound in H.
+    exists (match H in _ = z return firstn _ tus ++ z = tus with
+              | eq_refl => firstn_skipn _ _
+            end).
+    intros.
+    generalize (firstn_skipn (length tus - length ts) tus).
+    generalize dependent (skipn (length tus - length ts) tus).
+    generalize dependent (firstn (length tus - length ts) tus).
+    intros; subst. simpl. rewrite hlist_split_hlist_app.
+    reflexivity.
+  Qed.
+
+  Global Instance Injective_WellFormed_ctx_subst tus tvs c t s
+  : Injective (WellFormed_ctx_subst tus tvs (AllSubst (c:=c) (t:=t) s)) :=
+    { result := exists tvs', tvs = tvs' ++ t :: nil /\
+                             WellFormed_ctx_subst tus tvs' s }.
+  Proof. admit. Defined.
+
+  SearchAbout Injective.
+
+  Global Instance Injective_app_cons {T} (a : list T) b c d
+  : Injective (a ++ b :: nil = (c ++ d :: nil)) :=
+    { result := a = c /\ b = d }.
+  Proof. admit. Defined.
+
+  Theorem ctx_substD_lookup ctx
+  : forall (s : ctx_subst ctx) (uv : nat) (e : expr),
+      ctx_lookup uv s = Some e ->
+      forall (tus tvs : tenv typ),
+        WellFormed_ctx_subst (tus ++ getUVars ctx) (tvs ++ getVars ctx)  s ->
+        forall  (sD : exprT tus tvs Prop),
+        ctx_substD tus tvs s = Some sD ->
+        exists (t : typ) (val : exprT tus tvs (typD t))
+               (get : hlist typD tus -> typD t),
+          nth_error_get_hlist_nth typD tus uv =
+          Some (existT (fun t0 : typ => hlist typD tus -> typD t0) t get) /\
+          exprD' tus tvs e t = Some val /\
+          (forall (us : hlist typD tus) (vs : hlist typD tvs),
+             sD us vs -> get us = val us vs).
+  Proof.
+    induction s; simpl; intros.
+    { congruence. }
+    { forward; inv_all; subst.
+      inv_all.
+      eapply drop_exact_sound in H2.
+      forward_reason.
+      revert H1. subst.
+      (*
+      generalize x1. intro; inv_all; subst.
+      specialize (IHs _ _ H _ _ H6 _ H3).
+      forward_reason.
+      eapply exprD'_weakenV with (tvs' := t :: nil) in H4; eauto.
+      forward_reason.
+      do 3 eexists; split; eauto. split; eauto.
+      intros. revert H8.
+      rewrite <- (hlist_app_hlist_split _ _ vs). intro.
+      rewrite <- H7; clear H7.
+      eapply H5.
+      specialize (H0 (fst (hlist_split x0 (t :: nil) vs))
+                     (snd (hlist_split x0 (t :: nil) vs))).
+      generalize dependent (hlist_app (fst (hlist_split x0 (t :: nil) vs))
+               (snd (hlist_split x0 (t :: nil) vs))). *)
+      admit. }
+    { admit. }
+    { admit. (*forward; inv_all; subst.
+      consider (UVarMap.MAP.find uv s'); intros; inv_all; subst.
+      { eapply SUBST.substD_lookup in H2; eauto.
+        forward_reason.
+        do 3 eexists; split; eauto. split; eauto.
+        intros. destruct H8. eauto. }
+      { eapply IHWellFormed_ctx_subst in H3; eauto.
+        forward_reason.
+        eapply drop_exact_sound in H4.
+        forward_reason.
+        revert H4. subst tus; intros.
+        exists x0.
+        eapply nth_error_get_hlist_nth_weaken with (ls' := t) in H3.
+        simpl in *. forward_reason.
+        eapply exprD'_weakenU with (tus' := t) in H7; eauto.
+        forward_reason.
+        do 2 eexists; split; eauto; split; eauto.
+        do 2 intro.
+        rewrite <- (hlist_app_hlist_split _ _ us).
+        rewrite <- H9; clear H9.
+        rewrite <- H10; clear H10. destruct 1.
+        eapply H8. rewrite H4 in H10. assumption. } *) }
+  Qed.
+
+  Lemma ctx_subst_domain ctx tus tvs
+  : forall (s : ctx_subst ctx),
+      WellFormed_ctx_subst tus tvs s ->
+      forall (ls : list nat),
+      subst_domain s = ls ->
+      forall n : nat, In n ls <-> subst_lookup n s <> None.
+  Proof.
+    induction 1; simpl; intros; eauto using WellFormed_domain.
+    { subst. split; auto. congruence. }
+    { subst. rewrite in_app_iff.
+      split; intro.
+      { forward.
+        destruct H2.
+        { eapply IHWellFormed_ctx_subst in H2; eauto. }
+        { eapply SUBST.WellFormed_domain in H2; eauto. } }
+      { rewrite IHWellFormed_ctx_subst; eauto.
+        rewrite SUBST.WellFormed_domain; eauto.
+        unfold SUBST.raw_lookup, amap_lookup in *.
+        destruct (UVarMap.MAP.find n s'); eauto. } }
+  Qed.
+
+  Global Instance SubstOk_cxt_subst tus tvs ctx
+  : @SubstOk (ctx_subst ctx) typ expr _ _ _ :=
+  { WellFormed_subst := @WellFormed_ctx_subst ctx (tus ++ getUVars ctx) (tvs ++ getVars ctx)
+  ; substD := @ctx_substD _
+  }.
+  { intros. eapply ctx_substD_lookup in H; eauto. eapply H0. auto. }
+  { intros; eapply ctx_subst_domain; eauto. }
+  { admit. }
+  Defined.
+
+  Global Instance SubstUpdate_ctx_subst ctx
+  : SubstUpdate (ctx_subst ctx) expr :=
+  { subst_set := ctx_set
+  ; subst_empty := ctx_empty
+  }.
+
+  Definition propD := @exprD'_typ0 _ _ _ _ Prop _.
+
+  Fixpoint pctxD (tus tvs : tenv typ) (ctx : Ctx) (s : ctx_subst ctx) {struct s}
+  : option (   exprT (tus ++ getUVars ctx) (tvs ++ getVars ctx) Prop
+            -> exprT tus tvs Prop) :=
+    match s in ctx_subst ctx
+          return option (   exprT (tus ++ getUVars ctx) (tvs ++ getVars ctx) Prop
+                         -> exprT tus tvs Prop)
+    with
+      | TopSubst =>
+        Some (fun k us vs => k (hlist_app us Hnil) (hlist_app vs Hnil))
+      | AllSubst t ctx' s' =>
+        match pctxD tus tvs s' with
+          | Some cD =>
+            Some (fun k : exprT _ _ Prop =>
+                    cD (fun us vs =>
+                          forall x : typD t,
+                            k us
+                              match
+                                app_ass_trans tvs (getVars ctx') (t :: nil) in (_ = t0)
+                                return (hlist typD t0)
+                              with
+                                | eq_refl => hlist_app vs (Hcons x Hnil)
+                              end))
+          | None => None
+        end
+      | ExsSubst ts ctx' s' sub =>
+        match SUBST.raw_substD ((tus ++ getUVars ctx') ++ ts) (tvs ++ getVars ctx') sub
+            , pctxD tus tvs s'
+        with
+          | Some sD , Some cD =>
+            Some (fun k : exprT (tus ++ getUVars ctx' ++ ts) (tvs ++ getVars ctx') Prop =>
+                    cD (fun us vs =>
+                          _foralls typD ts (fun us' =>
+                                             sD (hlist_app us us') vs ->
+                                             k match
+                                                 app_ass_trans tus _ ts in (_ = t0)
+                                                 return (hlist typD t0)
+                                               with
+                                                 | eq_refl => hlist_app us us'
+                                               end
+                                               vs)))
+          | _ , _ => None
+        end
+      | HypSubst h ctx' s' =>
+        match propD (tus ++ getUVars ctx') (tvs ++ getVars ctx') h with
+          | None => None
+          | Some pD => match pctxD tus tvs s' with
+                         | None => None
+                         | Some cD =>
+                           Some (fun k : exprT _ _ Prop =>
+                                   cD (fun us vs => pD us vs -> k us vs))
+                       end
+        end
+    end.
+
+  Definition RCtx {tus tvs tus' tvs'} :=
+    (RexprT tus tvs Basics.impl ==> RexprT tus' tvs' Basics.impl)%signature.
+
+  Local Existing Instance Transitive_Roption.
+  Local Existing Instance Symmetric_Roption.
+  Local Existing Instance Reflexive_Roption.
+  Local Existing Instance Transitive_RexprT.
+  Local Existing Instance Symmetric_RexprT.
+  Local Existing Instance Reflexive_RexprT.
+
+  Theorem Proper_pctxD_iff
+  : forall tus tvs c1 s,
+      Proper (Roption (RexprT (tus ++ getUVars c1) (tvs ++ getVars c1) iff ==>
+                              (RexprT tus tvs iff)))%signature
+             (@pctxD tus tvs c1 s).
+  Proof.
+    induction s; simpl; intros.
+    { constructor.
+      do 6 red; simpl; intros.
+      eapply H; rewrite <- equiv_hlist_app; split; auto; constructor. }
+    { red; simpl.
+      destruct (pctxD tus tvs s); try constructor.
+      inv_all.
+      do 6 red. intros.
+      eapply IHs; eauto.
+      do 5 red; intros.
+      eapply forall_iff. intros.
+      eapply H; eauto.
+      equivs. reflexivity. }
+    { repeat match goal with
+               | |- context [ match ?X with _ => _ end ] => destruct X ; try constructor
+             end.
+      red; intros.
+      inv_all. eapply IHs.
+      do 5 red; intros.
+      apply equiv_eq_eq in H0.
+      apply equiv_eq_eq in H1. subst.
+      eapply impl_iff. reflexivity.
+      intro. eapply H; reflexivity. }
+    { repeat match goal with
+               | |- context [ match ?X with _ => _ end ] => destruct X ; try solve [ constructor ]
+             end.
+      constructor.
+      inv_all; do 6 red; intros.
+      equivs.
+      eapply IHs; try reflexivity.
+      do 5 red; intros; equivs.
+      eapply _forall_iff. intros.
+      eapply impl_iff. reflexivity.
+      intro. eapply H; reflexivity. }
+  Qed.
+
+  Theorem Proper_pctxD_impl
+  : forall tus tvs c1 s,
+      Proper (Roption (RexprT (tus ++ getUVars c1) (tvs ++ getVars c1) Basics.impl ==>
+                              (RexprT tus tvs Basics.impl)))%signature
+             (@pctxD tus tvs c1 s).
+  Proof.
+    induction s; simpl; intros.
+    { constructor.
+      do 6 red; intros.
+      eapply H; rewrite <- equiv_hlist_app; split; auto; constructor. }
+    { red; simpl.
+      destruct (pctxD tus tvs s); try constructor.
+      inv_all.
+      do 7 red. intros.
+      eapply IHs; eauto.
+      do 6 red; intros.
+      equivs.
+      eapply H; eauto; reflexivity. }
+    { repeat match goal with
+               | |- context [ match ?X with _ => _ end ] => destruct X ; try constructor
+             end.
+      red; intros.
+      inv_all. eapply IHs.
+      do 6 red; intros.
+      equivs.
+      eapply H; eauto; reflexivity. }
+    { repeat match goal with
+               | |- context [ match ?X with _ => _ end ] => destruct X ; try solve [ constructor ]
+             end.
+      constructor.
+      inv_all.
+      do 7 red; intros.
+      eapply IHs; eauto.
+      do 6 red; intros.
+      equivs.
+      eapply _forall_sem; intro.
+      eapply _forall_sem with (x := x0) in H5.
+      intros. eapply H; eauto; reflexivity. }
+  Qed.
+
+  Theorem Applicative_pctxD
+  : forall tus tvs ctx s C,
+      @pctxD tus tvs ctx s = Some C ->
+      (forall us vs (P Q : exprT _ _ Prop),
+         C (fun a b => P a b -> Q a b) us vs ->
+         C P us vs ->
+         C Q us vs) /\
+      (forall us vs (Q : exprT _ _ Prop), (forall a b, Q a b) -> C Q us vs).
+  Proof.
+    clear. induction s; simpl; intros.
+    { forward; inv_all; subst.
+      forward_reason; split; eauto. }
+    { forward; inv_all; subst.
+      destruct (IHs _ eq_refl) as [ Hap Hpure ]; clear IHs.
+      generalize (Proper_pctxD_impl tus tvs s).
+      Cases.rewrite_all_goal.
+      intros; inv_all.
+      split.
+      { intros us vs P Q f.
+        eapply Hap.
+        eapply H0; [ | reflexivity | reflexivity | eapply f ].
+        simpl. clear.
+        do 6 red. intros; equivs; eauto. }
+      { intros us vs Q v.
+        eapply Hpure. intros; eauto. } }
+    { forward; inv_all; subst.
+      destruct (IHs _ eq_refl) as [ Hap Hpure ]; clear IHs.
+      generalize (Proper_pctxD_impl tus tvs s).
+      Cases.rewrite_all_goal; intros; inv_all.
+      split.
+      { intros us vs P Q f.
+        eapply Hap.
+        eapply H1; [ | reflexivity | reflexivity | eapply f ].
+        clear.
+        do 6 red; intros; equivs.
+        tauto. }
+      { intros. eapply Hpure.
+        intros. eauto. } }
+    { forward; inv_all; subst.
+      destruct (IHs _ eq_refl) as [ Hap Hpure ]; clear IHs.
+      generalize (Proper_pctxD_impl tus tvs s).
+      Cases.rewrite_all_goal.
+      intros; inv_all.
+      split.
+      { rename P into P0.
+        intros us vs P Q f.
+        eapply Hap.
+        eapply H1; [ | reflexivity | reflexivity | eapply f ].
+        simpl. clear.
+        do 6 red. intros; equivs; eauto.
+        eapply _forall_sem. intros.
+        rewrite _forall_sem in H2.
+        rewrite _forall_sem in H1.
+        eauto. }
+      { intros us vs Q v.
+        eapply Hpure. intros.
+        eapply _forall_sem; intros.
+        eauto. } }
+  Qed.
+
+  Lemma Ap_pctxD
+  : forall tus tvs (ctx : Ctx) (s : ctx_subst ctx)
+           (C : exprT (tus ++ getUVars ctx) (tvs ++ getVars ctx) Prop ->
+                exprT tus tvs Prop),
+      pctxD tus tvs s = Some C ->
+      forall (us : hlist typD tus) (vs : hlist typD tvs)
+             (P Q : exprT (tus ++ getUVars ctx) (tvs ++ getVars ctx) Prop),
+        C (fun us vs => P us vs -> Q us vs) us vs -> C P us vs -> C Q us vs.
+  Proof.
+    intros. revert H1. revert H0. eapply Applicative_pctxD in H; eauto.
+    destruct H. eapply H.
+  Qed.
+
+  Lemma Pure_pctxD
+  : forall tus tvs (ctx : Ctx) (s : ctx_subst ctx)
+           (C : exprT (tus ++ getUVars ctx) (tvs ++ getVars ctx) Prop ->
+                exprT tus tvs Prop),
+      pctxD tus tvs s = Some C ->
+      forall (P : exprT (tus ++ getUVars ctx) (tvs ++ getVars ctx) Prop),
+        (forall us vs, P us vs) -> forall us vs, C P us vs.
+  Proof.
+    intros. eapply Applicative_pctxD in H; eauto.
+    destruct H. eapply H1; eauto.
+  Qed.
+
+  Definition CtxMorphism {tus tvs tus' tvs'}
+             (c1 c2 : exprT tus tvs Prop -> exprT tus' tvs' Prop) : Prop :=
+    forall (P : exprT _ _ Prop) us vs, c1 P us vs -> c2 P us vs.
+
+  Inductive SubstMorphism (tus tvs : tenv typ)
+  : forall c : Ctx, ctx_subst c -> ctx_subst c -> Prop :=
+  | SMall : forall c t s1 s2,
+              @SubstMorphism tus tvs c s1 s2 ->
+              @SubstMorphism tus tvs (CAll c t) (AllSubst s1) (AllSubst s2)
+  | SMexs : forall c ts s1 s2 cs1 cs2,
+              (match @pctxD tus tvs c cs1
+                   , SUBST.raw_substD ((tus ++ getUVars c) ++ ts) (tvs ++ getVars c) s1
+                   , @pctxD tus tvs c cs2
+                   , SUBST.raw_substD ((tus ++ getUVars c) ++ ts) (tvs ++ getVars c) s2
+               with
+                 | None , _ , _ , _
+                 | Some _ , None , _ , _ => True
+                 | Some _ , Some _ , None , _
+                 | Some _ , Some _ , Some _ , None => False
+                 | Some c1D , Some s1D , Some c2D , Some s2D =>
+                   forall us vs, c2D (fun us vs =>
+                                       forall us',
+                                         s2D (hlist_app us us') vs ->
+                                         s1D (hlist_app us us') vs) us vs
+               end) ->
+              @SubstMorphism tus tvs c cs1 cs2 ->
+              @SubstMorphism tus tvs (CExs c ts) (ExsSubst cs1 s1) (ExsSubst cs2 s2)
+  | SMhyp : forall c h s1 s2,
+              @SubstMorphism tus tvs c s1 s2 ->
+              @SubstMorphism tus tvs (CHyp c h) (HypSubst s1) (HypSubst s2)
+  | SMtop : @SubstMorphism tus tvs CTop TopSubst TopSubst.
+
+  Lemma Fmap_pctxD_impl
+  : forall tus tvs c s C,
+      @pctxD tus tvs c s = Some C ->
+      Proper (RexprT _ _ Basics.impl ==> RexprT tus tvs Basics.impl)%signature C.
+  Proof.
+    clear. intros.
+    generalize (@Proper_pctxD_impl tus tvs c s).
+    rewrite H. intros; inv_all. auto.
+  Qed.
+
+  Lemma Fmap_pctxD_iff
+  : forall tus tvs c s C,
+      @pctxD tus tvs c s = Some C ->
+      Proper (RexprT _ _ iff ==> RexprT tus tvs iff)%signature C.
+  Proof.
+    clear. intros.
+    generalize (@Proper_pctxD_iff tus tvs c s).
+    rewrite H. intros; inv_all. auto.
+  Qed.
+
+  Lemma pctxD_SubstMorphism
+  : forall tus tvs ctx s s',
+      @SubstMorphism tus tvs ctx s s' ->
+      forall C C',
+      @pctxD tus tvs ctx s = Some C ->
+      @pctxD tus tvs ctx s' = Some C' ->
+      forall us vs (P : exprT _ _ Prop),
+        C P us vs -> C' P us vs.
+  Proof.
+    clear instantiate.
+    induction 1; intros; simpl in *; forward; inv_all; subst; eauto.
+    { eapply IHSubstMorphism; eauto. }
+    { simpl in *.
+      eapply (IHSubstMorphism _ _ eq_refl eq_refl) in H3.
+      destruct (Applicative_pctxD _ H2) as [ Hap Hpure ].
+      revert H3. eapply Hap.
+      generalize (H7 us vs).
+      eapply Hap.
+      eapply Hpure.
+      clear. intros.
+      rewrite _forall_sem.
+      rewrite _forall_sem in H0.
+      intros; eauto. }
+    { eapply IHSubstMorphism; eauto. }
+  Qed.
+
+  Definition fromAll {c t} (cs : ctx_subst (CAll c t)) : ctx_subst c :=
+    match cs in ctx_subst c
+          return match c with
+                   | CAll c _ => ctx_subst c
+                   | _ => unit
+                 end
+    with
+      | AllSubst _ _ c => c
+      | _ => tt
+    end.
+
+  Definition fromHyp {c t} (cs : ctx_subst (CHyp c t)) : ctx_subst c :=
+    match cs in ctx_subst c
+          return match c with
+                   | CHyp c _ => ctx_subst c
+                   | _ => unit
+                 end
+    with
+      | HypSubst _ _ c => c
+      | _ => tt
+    end.
+
+  Definition fromExs {c t} (cs : ctx_subst (CExs c t)) : subst * ctx_subst c :=
+    match cs in ctx_subst c
+          return match c with
+                   | CExs c _ => subst * ctx_subst c
+                   | _ => unit
+                 end
+    with
+      | ExsSubst _ _ c s => (s,c)
+      | _ => tt
+    end.
+
+  Global Instance Injective_SubstMorphism_AllSubst tus tvs t ctx s s'
+  : Injective (@SubstMorphism tus tvs (CAll ctx t) (AllSubst s) s') :=
+  { result := exists s'', s' = AllSubst s'' /\ @SubstMorphism tus tvs ctx s s'' }.
+  intros.
+  exists (fromAll s').
+  refine
+    (match H in @SubstMorphism _ _ C X Y
+           return match X in ctx_subst C' return ctx_subst C' -> Prop with
+                    | AllSubst t s c => fun s' =>
+                                            s' = AllSubst (fromAll s') /\
+                                            SubstMorphism tus tvs c (fromAll s')
+                    | _ => fun _ => True
+                  end Y
+     with
+       | SMall _ _ _ _ _ => _
+       | _ => I
+     end).
+  simpl; eauto.
+  Defined.
+
+  Global Instance Injective_SubstMorphism_HypSubst tus tvs t ctx s s'
+  : Injective (@SubstMorphism tus tvs (CHyp ctx t) (HypSubst s) s') :=
+  { result := exists s'', s' = HypSubst s'' /\ @SubstMorphism tus tvs ctx s s'' }.
+  intros.
+  exists (fromHyp s').
+  refine
+    (match H in @SubstMorphism _ _ C X Y
+           return match X in ctx_subst C' return ctx_subst C' -> Prop with
+                    | HypSubst t s c => fun s' =>
+                                            s' = HypSubst (fromHyp s') /\
+                                            SubstMorphism tus tvs c (fromHyp s')
+                    | _ => fun _ => True
+                  end Y
+     with
+       | SMhyp _ _ _ _ _ => _
+       | _ => I
+     end).
+  simpl; eauto.
+  Defined.
+
+  Global Instance Injective_SubstMorphism_TopSubst tus tvs s'
+  : Injective (@SubstMorphism tus tvs CTop TopSubst s') :=
+  { result := s' = TopSubst }.
+  Proof.
+    intros.
+    refine
+      (match H in @SubstMorphism _ _ C X Y
+             return match X in ctx_subst C' return ctx_subst C' -> Prop with
+                      | TopSubst => fun s' => s' = TopSubst
+                      | _ => fun _ => True
+                    end Y
+       with
+         | SMtop => eq_refl
+         | _ => I
+       end).
+  Defined.
+
+  Global Instance Injective_SubstMorphism_ExsSubst tus tvs ctx tes s s' sub
+  : Injective (@SubstMorphism tus tvs (CExs ctx tes) (ExsSubst sub s) s') :=
+  { result := exists s'' sub',
+                s' = ExsSubst sub' s''
+                /\ (match @pctxD tus tvs ctx sub
+                        , SUBST.raw_substD ((tus ++ getUVars ctx) ++ tes) (tvs ++ getVars ctx) s
+                        , @pctxD tus tvs ctx sub'
+                        , SUBST.raw_substD ((tus ++ getUVars ctx) ++ tes) (tvs ++ getVars ctx) s''
+                    with
+                      | None , _ , _ , _
+                      | Some _ , None , _ , _ => True
+                      | Some _ , Some _ , None , _
+                      | Some _ , Some _ , Some _ , None => False
+                      | Some c1D , Some s1D , Some c2D , Some s2D =>
+                        forall us vs, c2D (fun us vs =>
+                                             forall us',
+                                               s2D (hlist_app us us') vs ->
+                                               s1D (hlist_app us us') vs) us vs
+                    end)
+                /\ SubstMorphism tus tvs sub sub'}.
+  intros. exists (fst (fromExs s')). exists (snd (fromExs s')).
+  refine
+    (match H in @SubstMorphism _ _ C X Y
+           return match X in ctx_subst C' return ctx_subst C' -> Prop with
+                    | ExsSubst t s su c =>
+                      fun s' =>
+                        s' = ExsSubst (snd (fromExs s')) (fst (fromExs s')) /\
+                        match pctxD tus tvs su with
+                          | Some _ =>
+                            match
+                              SUBST.raw_substD ((tus ++ getUVars s) ++ t) (tvs ++ getVars s) c
+                            with
+                              | Some s1D =>
+                                match pctxD tus tvs (snd (fromExs s')) with
+                                  | Some c2D =>
+                                    match
+                                      SUBST.raw_substD ((tus ++ getUVars s) ++ t)
+                                             (tvs ++ getVars s) (fst (fromExs s'))
+                                    with
+                                      | Some s2D =>
+                                        forall us vs,
+                                          c2D
+                                            (fun us0 vs0 =>
+                                               forall us' : hlist typD t,
+                                                 s2D (hlist_app us0 us') vs0 ->
+                                                 s1D (hlist_app us0 us') vs0) us vs
+                                      | None => False
+                                    end
+                                  | None => False
+                                end
+                              | None => True
+                            end
+                          | None => True
+                        end /\
+                        SubstMorphism tus tvs su (snd (fromExs s'))
+                    | _ => fun _ => True
+                  end Y
+     with
+       | SMexs _ _ _ _ _ _ _ _ => _
+       | _ => I
+     end).
+  simpl; eauto.
+  Defined.
+
+  Global Instance Reflexive_SubstMorphism tus tvs ctx
+  : Reflexive (@SubstMorphism tus tvs ctx).
+  Proof.
+    red. induction x;
+         simpl; intros; try constructor;
+         forward; eauto.
+    eapply Applicative_pctxD; eauto.
+  Qed.
+
+  Global Instance Transitive_SubstMorphism tus tvs ctx
+  : Transitive (@SubstMorphism tus tvs ctx).
+  Proof.
+    red. intros x y z H; revert z.
+    induction H.
+    { intros; inv_all; subst.
+      constructor; eauto. }
+    { intros; inv_all; subst.
+      forward. simpl in *.
+      constructor.
+      { forward. inv_all; subst.
+        Cases.rewrite_all_goal.
+        repeat match goal with
+                 | H : ?X = _ , H' : ?X = _ |- _ =>
+                   rewrite H in H'
+               end; inv_all; subst.
+        specialize (H8 us vs).
+        specialize (H6 us vs).
+        revert H8.
+        eapply (Applicative_pctxD _ H5).
+        eapply (pctxD_SubstMorphism H4 H1 H5 us vs).
+        revert H6.
+        eapply (Fmap_pctxD_impl _ H1); try reflexivity.
+        clear.
+        do 6 red. intros. equivs. firstorder. }
+      { eapply IHSubstMorphism. eassumption. } }
+    { intros; inv_all; subst. constructor; eauto. }
+    { intros; inv_all; subst.
+      constructor. }
+  Qed.
+
+End parameterized.
+
+Arguments CTop {typ expr} : rename.
+Arguments CEx {typ expr} _ _ : rename.
+Arguments CAll {typ expr} _ _ : rename.
+Arguments CHyp {typ expr} _ _ : rename.
+
+Export MirrorCore.ExprI.
+Export MirrorCore.ExprDAs.
